src/Assembly/Proofs.v
@@ -1,0 +1,308 @@
+Require Import Coq.Lists.List.
+Require Import Coq.NArith.NArith.
+Require Import Coq.ZArith.ZArith.
+Require Import Crypto.Language.API.
+Require Import Crypto.Language.APINotations.
+Require Import Crypto.AbstractInterpretation.ZRange.
+Require Import Crypto.Util.ErrorT.
+Require Import Crypto.Assembly.Syntax.
+Require Import Crypto.Assembly.Semantics.
+Require Import Crypto.Assembly.Symbolic.
+Require Import Crypto.Assembly.Equivalence.
+Require Import Crypto.Util.Option.
+Require Import Crypto.Util.Notations.
+Require Import Crypto.Util.Sum.
+Require Import Crypto.Util.Bool.Reflect.
+Require Import Crypto.Util.Tactics.BreakMatch.
+Require Import Crypto.Util.Tactics.DestructHead.
+Import API.Compilers APINotations.Compilers AbstractInterpretation.ZRange.Compilers.
+Import ListNotations.
+Local Open Scope list_scope.
+
+(*
+Require Import Crypto.Assembly.Parse.
+Require Import Crypto.Util.Strings.String.
+Require Import Crypto.Stringification.Language.
+Require Import Crypto.Util.Strings.Show.
+Require Import Crypto.Util.Option.
+Require Import Crypto.Util.OptionList.
+Import API.Compilers APINotations.Compilers AbstractInterpretation.ZRange.Compilers.
+Local Open Scope string_scope.
+ *)
+Fixpoint eval_base_var (dag : dag) {t : base.type} : base_var t -> API.interp_type (type.base t) -> Prop :=
+  match t with
+  | base.type.unit => fun _ _ => True
+  | base.type.type_base base.type.Z => fun idx v => exists n, Z.of_N n = v /\ eval dag (ExprRef idx) n
+  | base.type.prod _ _ => fun a b => eval_base_var dag (fst a) (fst b) /\ eval_base_var dag (snd a) (snd b)
+  | base.type.list _ => List.Forall2 (eval_base_var dag)
+  | base.type.type_base base.type.nat => @eq _
+  | base.type.type_base base.type.zrange => @eq _
+  | _ => fun _ _ => False
+  end%bool.
+
+Definition eval_var (dag : dag) {t : API.type} : var t -> API.interp_type t -> Prop
+  := match t with
+     | type.base _ => eval_base_var dag
+     | type.arrow _ _ => fun _ _ => False
+     end.
+
+Check @symex_expr.
+Print symex_T.
+(* TODO(Jason?): figure out this lemma statement, reduce proof to ident case *)
+(*Theorem symex_expr_correct
+        {t} (expr : API.Expr t)
+  : ???.
+ *)
+Theorem symex_PHOAS_PHOAS_correct
+        {t} (expr : API.Expr t)
+        (input_var_data : type.for_each_lhs_of_arrow var t)
+        (d : dag)
+        (rets : base_var (type.final_codomain t))
+        (d' : dag)
+        (Hwf : API.Wf expr)
+        (H : symex_PHOAS_PHOAS expr input_var_data d = Success (rets, d'))
+        (d_ok : dag_ok d)
+  : (forall (input_runtime_var : type.for_each_lhs_of_arrow API.interp_type t),
+        type.and_for_each_lhs_of_arrow (@eval_var d) input_var_data input_runtime_var
+        -> eval_base_var d' rets (type.app_curried (API.Interp expr) input_runtime_var))
+    /\ dag_ok d'
+    /\ (forall e n, eval d e n -> eval d' e n).
+Proof.
+  cbv [symex_PHOAS_PHOAS] in H.
+  (* TODO(Jason): Prove this from [symex_expr_correct] *)
+Admitted.
+
+Definition eval_idx_Z (dag : dag) (idx : idx) (v : Z) : Prop
+  := exists n, Z.of_N n = v /\ eval dag (ExprRef idx) n.
+Definition eval_idx_or_list_idx (d : dag) (v1 : idx + list idx) (v2 : Z + list Z)
+  : Prop
+  := match v1, v2 with
+     | inl idx, inl v => eval_idx_Z d idx v
+     | inr idxs, inr vs => Forall2 (eval_idx_Z d) idxs vs
+     | inl _, inr _ | inr _, inl _ => False
+     end.
+
+Fixpoint build_base_runtime (t : base.type) (values : list (Z + list Z))
+  : option (base.interp t * list (Z + list Z))
+  := match t, values return option (base.interp t * list (Z + list Z)) with
+     | base.type.unit, _
+       => Some (tt, values)
+     | base.type.type_base base.type.Z, inl val :: values
+       => Some (val, values)
+     | base.type.prod A B, _
+       => (vA <- build_base_runtime A values;
+          let '(vA, values) := vA in
+          vB <- build_base_runtime B values;
+          let '(vB, values) := vB in
+          Some ((vA, vB), values))
+     | base.type.list (base.type.type_base base.type.Z), inr value :: values
+       => Some (value, values)
+     | base.type.type_base base.type.Z, inr _ :: _
+     | base.type.list (base.type.type_base base.type.Z), inl _ :: _
+     | base.type.type_base _, []
+     | base.type.list _, []
+     | base.type.type_base _, _
+     | base.type.option _, _
+     | base.type.list _, _ :: _
+       => None
+     end%option.
+Definition build_runtime (t : API.type) (values : list (Z + list Z))
+  : option (API.interp_type t * list (Z + list Z))
+  := match t with
+     | type.base t => build_base_runtime t values
+     | type.arrow _ _ => None
+     end.
+Fixpoint build_input_runtime (t : API.type) (values : list (Z + list Z))
+  : option (type.for_each_lhs_of_arrow API.interp_type t * list (Z + list Z))
+  := match t with
+     | type.base _ => Some (tt, values)
+     | type.arrow A B
+       => (vA <- build_runtime A values;
+          let '(vA, values) := vA in
+          vB <- build_input_runtime B values;
+          let '(vB, values) := vB in
+          Some ((vA, vB), values))
+     end%option.
+
+Fixpoint simplify_base_runtime {t : base.type} : base.interp t -> option (list (Z + list Z))
+  := match t return base.interp t -> option (list (Z + list Z)) with
+     | base.type.unit
+       => fun 'tt => Some []
+     | base.type.type_base base.type.Z => fun val => Some [inl val]
+     | base.type.prod A B => fun ab => (a <- simplify_base_runtime (fst ab); b <- simplify_base_runtime (snd ab); Some (a ++ b))
+     | base.type.list (base.type.type_base base.type.Z)
+       => fun ls : list Z => Some (List.map inl ls)
+     | base.type.list _
+     | base.type.type_base _
+     | base.type.option _
+       => fun _ => None
+     end%option.
+
+Theorem symex_PHOAS_correct
+        {t} (expr : API.Expr t)
+        (inputs : list (idx + list idx))
+        (d : dag)
+        (rets : list (idx + list idx))
+        (d' : dag)
+        (Hwf : API.Wf expr)
+        (H : symex_PHOAS expr inputs d = Success (rets, d'))
+        (d_ok : dag_ok d)
+        (t_ok : type_ok t)
+  : (forall (runtime_inputs : list (Z + list Z)),
+        List.Forall2 (eval_idx_or_list_idx d) inputs runtime_inputs
+        -> exists (input_runtime_var : type.for_each_lhs_of_arrow API.interp_type t)
+                  (runtime_rets : list (Z + list Z)),
+          build_input_runtime t runtime_inputs = Some (input_runtime_var, [])
+          /\ simplify_base_runtime (type.app_curried (API.Interp expr) input_runtime_var) = Some runtime_rets
+          /\ List.Forall2 (eval_idx_or_list_idx d') rets runtime_rets)
+    /\ dag_ok d'
+    /\ (forall e n, eval d e n -> eval d' e n).
+Proof.
+  cbv [symex_PHOAS ErrorT.bind] in H.
+  repeat first [ progress break_innermost_match_hyps
+               | progress destruct_head'_and
+               | progress subst
+               | discriminate
+               | assumption
+               | apply (f_equal (@Some _))
+               | apply (f_equal2 (@pair _ _))
+               | reflexivity
+               | progress reflect_hyps
+               | match goal with
+                 | [ H : Success _ = Success _ |- _ ] => inversion H; clear H
+                 | [ H : symex_PHOAS_PHOAS _ _ _ = _ |- _ ] => apply symex_PHOAS_PHOAS_correct in H; [ | assumption.. ]
+                 | [ |- exists a b, ?v = Some (a, _) /\ _ = Some b /\ _ ]
+                   => let av := fresh in destruct v as [ [av ?] |] eqn:?; [ exists av | exfalso ]
+                 | [ |- exists a, _ /\ ?v = Some a /\ _ ]
+                   => let av := fresh in destruct v as [ av |] eqn:?; [ exists av | exfalso ]
+                 | [ H : List.length ?l = 0%nat |- _ ] => is_var l; destruct l; cbn in H
+                 end
+               | apply conj
+               | progress intros ].
+  (** TODO: Jason can finish this proof, all that remains is matching up PHOAS types *)
+Admitted.
+
+Check symex_asm_func.
+Theorem symex_asm_func_correct
+        (d : dag) (gensym_st : gensym_state) (output_types : type_spec) (stack_size : nat)
+        (inputs : list (idx + list idx)) (reg_available : list REG) (asm : Lines)
+        (rets : list (idx + list idx))
+        (s : symbolic_state)
+        (H : symex_asm_func d gensym_st output_types stack_size inputs reg_available asm = Success (rets, s))
+        (d' := s.(dag_state))
+  : (forall (st : machine_state)
+            (runtime_inputs : list (Z + list Z)),
+        List.Forall2 (eval_idx_or_list_idx d) inputs runtime_inputs
+        -> exists st'
+                  (* ??? *) (*(input_runtime_var : type.for_each_lhs_of_arrow API.interp_type t)*)
+                  (runtime_rets : list (Z + list Z)),
+          DenoteLines st asm = Some st'
+          (*/\ build_input_runtime t runtime_inputs = Some (input_runtime_var, [])*)
+          (*/\ simplify_base_runtime (type.app_curried (API.Interp expr) input_runtime_var) = Some runtime_rets*)
+          /\ List.Forall2 (eval_idx_or_list_idx d') rets runtime_rets)
+    /\ dag_ok d'
+    /\ (forall e n, eval d e n -> eval d' e n).
+Proof.
+Admitted.
+
+Lemma build_inputs_ok d gensym_st v inputs d' gensym_st'
+      (d_ok : dag_ok d)
+      (H : build_inputs (d, gensym_st) v = (inputs, (d', gensym_st')))
+  : True (* Something about inputs *)
+    /\ dag_ok d'
+    /\ True (* something about gensym_st' *).
+Proof.
+Admitted.
+
+Axiom empty_dag_ok : dag_ok empty_dag.
+
+Check @check_equivalence.
+Theorem check_equivalence_correct
+        {assembly_calling_registers' : assembly_calling_registers_opt}
+        {assembly_stack_size' : assembly_stack_size_opt}
+        {assembly_output_first : assembly_output_first_opt}
+        {assembly_argument_registers_left_to_right : assembly_argument_registers_left_to_right_opt}
+        {t}
+        (asm : Lines)
+        (expr : API.Expr t)
+        (arg_bounds : type.for_each_lhs_of_arrow ZRange.type.option.interp t)
+        (out_bounds : ZRange.type.base.option.interp (type.final_codomain t))
+        (Hwf : API.Wf expr)
+        (H : check_equivalence asm expr arg_bounds out_bounds = Success tt)
+        (st : machine_state)
+        (PHOAS_args : type.for_each_lhs_of_arrow API.interp_type t)
+        (args : list (Z + list Z))
+        (Hargs : build_input_runtime t args = Some (PHOAS_args, []))
+        (HPHOAS_args : type.andb_bool_for_each_lhs_of_arrow (@ZRange.type.option.is_bounded_by) arg_bounds PHOAS_args = true)
+  (* TODO(Andres): write down something that relates [st] to args *)
+  : exists st'
+           (retvals : list (Z + list Z)),
+    DenoteLines st asm = Some st'
+    /\ simplify_base_runtime (type.app_curried (API.Interp expr) PHOAS_args) = Some retvals
+    /\ True (* TODO(andres): write down something that relates st' to retvals *).
+Proof.
+  cbv beta delta [check_equivalence ErrorT.bind] in H.
+  repeat match type of H with
+         | (let n := ?v in _) = _
+           => set v as n in H;
+                lazymatch type of H with
+                | (let n := ?v in ?rest) = ?rhs
+                  => change (match v with n => rest end = rhs) in H
+                end
+         | match ?v with Success n => @?S n | Error e => @?E e end = ?rhs
+           => let n := fresh n in
+              let e := fresh e in
+              destruct v as [n|e] eqn:?; [ change (S n = rhs) in H | change (E e = rhs) in H ];
+                cbv beta in H
+         | match ?v with pair a b => @?P a b end = ?rhs
+           => let a := fresh a in
+              let b := fresh b in
+              destruct v as [a b] eqn:?; change (P a b = rhs) in H;
+                cbv beta in H
+         end; try discriminate; [].
+  subst.
+  pose proof empty_dag_ok.
+  repeat match goal with
+         | [ H : build_inputs _ _ = _ |- _ ] => move H at bottom; apply build_inputs_ok in H; [ | assumption.. ]
+         | [ H : symex_PHOAS _ _ _ = Success _ |- _ ] => move H at bottom; apply symex_PHOAS_correct in H; [ | assumption.. ]
+         | [ H : _ /\ _ |- _ ] => move H at bottom; destruct H
+         end.
+  epose (DenoteLines st asm).
+
+   lazymatch goal with
+   | [ H : symex_PHOAS _ _ _ = Success _ |- _ ] => apply symex_PHOAS_correct in H; [ | try assumption.. ]
+   end.
+  2: { move d0 at bottom.
+       Search empty_dag dag_ok.
+Admitted.
+
+Check @generate_assembly_of_hinted_expr.
+Theorem generate_assembly_of_hinted_expr_correct
+        {assembly_calling_registers' : assembly_calling_registers_opt}
+        {assembly_stack_size' : assembly_stack_size_opt}
+        {assembly_output_first : assembly_output_first_opt}
+        {assembly_argument_registers_left_to_right : assembly_argument_registers_left_to_right_opt}
+        {t}
+        (asm : Lines)
+        (expr : API.Expr t)
+        (f : type.interp _ t)
+        (arg_bounds : type.for_each_lhs_of_arrow ZRange.type.option.interp t)
+        (out_bounds : ZRange.type.base.option.interp (type.final_codomain t))
+        (asm_out : Lines)
+        (* Phrased this way to line up with the bounds pipeline exactly *)
+        (Hbounded
+         : (forall arg1 arg2
+                   (Harg12 : type.and_for_each_lhs_of_arrow (@type.eqv) arg1 arg2)
+                   (Harg1 : type.andb_bool_for_each_lhs_of_arrow (@ZRange.type.option.is_bounded_by) arg_bounds arg1 = true),
+               ZRange.type.base.option.is_bounded_by out_bounds (type.app_curried (API.Interp expr) arg1) = true
+               /\ type.app_curried (API.Interp expr) arg1 = type.app_curried f arg2)
+           /\ API.Wf expr)
+        (H : generate_assembly_of_hinted_expr asm expr arg_bounds out_bounds = Success asm_out)
+  : asm = asm_out
+    /\ True (* ??? Something about equivalence of [API.Interp expr] and [asm] *).
+Proof.
+  cbv [generate_assembly_of_hinted_expr] in H.
+  break_innermost_match_hyps; inversion H; subst; repeat apply conj; try reflexivity.
+Qed.
+
+(* Some theorems about the result of calling generate_assembly_of_hinted_expr_correct on various Pipeline functions *)
